added progress for choreography

semantics/proofs/deadlockFreedomScript.sml
@@ -1,7 +1,10 @@
-open preamble choreoUtilsTheory chorSemTheory chorPropsTheory
+open preamble choreoUtilsTheory chorSemTheory chorPropsTheory chorTypePropsTheory chorTypeTheory
+
+open typeSNTheory                                
 
 val _ = new_theory "deadlockFreedom";
 
+(*
 Theorem chor_deadlock_freedom:
   ∀c s.
    no_undefined_vars (s,c) ∧
@@ -38,8 +41,55 @@ Proof
   (* Recursion *)
   \\ metis_tac [trans_fix]
 QED
+*)
+
+Definition chorEnvsn_def:
+  chorEnvsn Γ Δ = (∀ p. envsn (localise Γ p) (localise Δ p))
+End
+
+Theorem richerLang_localise_sn:
+  chorEnvsn Γ s ∧ typecheck (localise Γ p) e t ⇒
+  (∃ cl v. eval_exp cl (localise s p) e = Value v ∧ sn_v t v) ∨
+  ∃ cl exn. eval_exp cl (localise s p) e = Exn exn
+Proof
+  rw[] >>
+  drule sn_lemma >> strip_tac >>
+  fs[sn_e_def, chorEnvsn_def] >>
+  ‘envsn (localise Γ p) (localise s p)’ by metis_tac[] >>
+  metis_tac[envsn_g_submap, DRESTRICT_SUBMAP, sn_exec_def]        
+QED
 
 Theorem chor_progress:
+  ∀c s. chorTypecheckOK Γ Θ c ∧ chorEnvtype Γ s ∧ chorEnvsn Γ s ⇒
+        ∃τ l s' c'. trans (s,c) (τ,l) (s',c') ∨ ¬not_finish c
 Proof
+  Cases >> rw [] >> rw [] >>
+  drule chortype_no_self_communication >> 
+  drule chortype_no_undefined_vars >> rpt strip_tac >>
+  first_x_assum $ drule_all_then $ strip_assume_tac >~
+  [‘IfThen v p c1 c2’, ‘(s, IfThen v p c1 c2)’]
+  >- (Cases_on `FLOOKUP s (v,p) = SOME (BoolV T)`
+     >- metis_tac [trans_if_true]
+     \\ Cases_on `FLOOKUP s (v,p)`
+      >- fs [no_undefined_vars_def,free_variables_def,FLOOKUP_DEF]
+      >> Cases_on ‘x = (BoolV F)’
+      >- metis_tac [trans_if_false]
+      >> metis_tac [not_BoolV, trans_if_exn]) >~
+  [‘Com p1 v1 p2 v2’]
+  >- (rename1 ‘Com p1 v1 p2 v2’
+     \\ `∃d. FLOOKUP s' (v1,p1) = SOME d`
+             by fs [no_undefined_vars_def,free_variables_def,FLOOKUP_DEF]
+      >> Cases_on ‘d’ 
+      \\ metis_tac [trans_com, trans_com_exn, no_self_comunication_def]) >~
+  [‘Let v p e c’, ‘(s,Let v p e c)’]
+  >- (gvs[chorTypecheckOK_let_thm] >> drule richerLang_localise_sn >> strip_tac >>      
+      ‘free_vars e ⊆ FDOM (localise s p)’ by metis_tac[typecheck_env_fv, chortype_localise_fdom, SUBSET_TRANS] >>
+      first_x_assum $ drule_all_then $ strip_assume_tac >>
+      metis_tac[trans_letval, trans_letexn])
+  (* Selection *)
+  >- metis_tac [trans_sel,no_self_comunication_def]
+  (* Recursion *)
+  \\ metis_tac [trans_fix]
+QED
 
 val _ = export_theory ()
